Fixed relative security definitions for MiniCET

Utils.v
@@ -62,3 +62,82 @@ Fixpoint remove_dupes {A : Type} (eqb : A -> A -> bool) (t : list A) : list A :=
                then      remove_dupes eqb xs
                else x :: remove_dupes eqb xs
   end.
+
+Definition prefix {X:Type} (xs ys : list X) : Prop :=
+  exists zs, List.app xs zs = ys.
+
+Lemma prefix_refl : forall {X:Type} {ds : list X},
+  prefix ds ds.
+Proof. intros X ds. exists []. apply app_nil_r. Qed.
+
+Lemma prefix_nil : forall {X:Type} (ds : list X),
+  prefix [] ds.
+Proof. intros X ds. unfold prefix. eexists. simpl. reflexivity. Qed.
+
+Lemma prefix_heads_and_tails : forall {X:Type} (h1 h2 : X) (t1 t2 : list X),
+  prefix (h1::t1) (h2::t2) -> h1 = h2 /\ prefix t1 t2.
+Proof.
+  intros X h1 h2 t1 t2. unfold prefix. intros Hpre.
+  destruct Hpre as [zs Hpre]; simpl in Hpre.
+  inversion Hpre; subst. eauto.
+Qed.
+
+Lemma prefix_heads : forall {X:Type} (h1 h2 : X) (t1 t2 : list X),
+  prefix (h1::t1) (h2::t2) -> h1 = h2.
+Proof.
+  intros X h1 h2 t1 t2 H. apply prefix_heads_and_tails in H; tauto.
+Qed.
+
+Lemma prefix_or_heads : forall {X:Type} (x y : X) (xs ys : list X),
+  prefix (x :: xs) (y :: ys) \/ prefix (y :: ys) (x :: xs) ->
+  x = y.
+Proof.
+  intros X x y xs ys H.
+  destruct H as [H | H]; apply prefix_heads in H; congruence.
+Qed.
+
+Lemma prefix_cons : forall {X:Type} (d :X) (ds1 ds2: list X),
+ prefix ds1 ds2 <->
+ prefix (d::ds1) (d::ds2).
+Proof.
+  intros X d ds1 ds2. split; [unfold prefix| ]; intros H.
+  - destruct H; subst.
+    eexists; simpl; eauto.
+  - apply prefix_heads_and_tails in H. destruct H as [_ H]. assumption.
+Qed.
+
+Lemma prefix_app : forall {X:Type} {ds1 ds2 ds0 ds3 : list X},
+  prefix (ds1 ++ ds2) (ds0 ++ ds3) ->
+  prefix ds1 ds0 \/ prefix ds0 ds1.
+Proof.
+  intros X ds1. induction ds1 as [| d1 ds1' IH]; intros ds2 ds0 ds3 H.
+  - left. apply prefix_nil.
+  - destruct ds0 as [| d0 ds0'] eqn:D0.
+    + right. apply prefix_nil.
+    + simpl in H; apply prefix_heads_and_tails in H.
+      destruct H as [Heq Hpre]; subst.
+      apply IH in Hpre; destruct Hpre; [left | right];
+      apply prefix_cons; assumption.
+Qed.
+
+Lemma prefix_append_front : forall {X:Type} {ds1 ds2 ds3 : list X},
+  prefix (ds1 ++ ds2) (ds1 ++ ds3) ->
+  prefix ds2 ds3.
+Proof.
+  intros X ds1. induction ds1 as [| d1 ds1' IH]; intros ds2 ds3 H.
+  - auto.
+  - simpl in H; apply prefix_cons in H. apply IH in H. assumption.
+Qed.
+
+Lemma app_eq_prefix : forall {X:Type} {ds1 ds2 ds1' ds2' : list X},
+  List.app ds1 ds2 = List.app ds1' ds2' ->
+  prefix ds1 ds1' \/ prefix ds1' ds1.
+Proof.
+  intros X ds1. induction ds1 as [| h1 t1 IH]; intros ds2 ds1' ds2' H.
+  - left. apply prefix_nil.
+  - destruct ds1' as [| h1' t1'] eqn:D1'.
+    + right. apply prefix_nil.
+    + simpl in H; inversion H; subst.
+      apply IH in H2. destruct H2 as [HL | HR];
+      [left | right]; apply prefix_cons; auto.
+Qed.
